lawyer/nonblocking/tokens/fundamental_tok.v
@@ -2,6 +2,7 @@
 (* From iris.program_logic Require Export weakestpre. *)
 
 From iris.proofmode Require Import proofmode coq_tactics.
+From lawyer.nonblocking Require Import op_eval_helpers.
 From lawyer.nonblocking.logrel Require Export persistent_pred substitutions valid_client stuck_utils.
 From lawyer.nonblocking.tokens Require Export logrel_tok.
 (* From lawyer.nonblocking Require Export pwp.  *)
@@ -22,44 +23,11 @@ Section typed_interp.
   
   Notation D := (persistent_predO val (iPropI Σ)).
   
-  Lemma bin_op_eval_inv op a b r
-    (EVAL: bin_op_eval op a b = Some r):
-    (op = EqOp /\ vals_compare_safe a b /\ r = LitV $ LitBool $ bool_decide (a = b)) \/
-    (exists na nb vr, a = LitV $ LitInt na /\ b = LitV $ LitInt nb /\ r = LitV vr /\
-                 ((exists i, vr = LitInt i) \/ (exists b, vr = LitBool b)) /\
-                 bin_op_eval_int op na nb = Some vr) \/
-    (exists ba bb br, a = LitV $ LitBool ba /\ b = LitV $ LitBool bb /\ r = LitV $ LitBool br /\
-                 bin_op_eval_bool op ba bb = Some $ LitBool br) \/
-    (exists la ob, a = LitV $ LitLoc la /\ b = LitV (LitInt ob) /\
-              op = OffsetOp /\
-              r = LitV (LitLoc (la +ₗ ob))).
-  Proof using.
-    rewrite /bin_op_eval in EVAL.
-    destruct decide.
-    { subst. destruct decide; [| done].
-      left. inversion EVAL. subst. eauto. }
-    destruct a; try done.
-    destruct l; try done.
-    all: destruct b; (try done); destruct l; try done.
-    - apply fmap_Some in EVAL as (?&?&->).
-      right. left. do 3 eexists. repeat split; eauto.
-      destruct op; simpl in H; set_solver.      
-    - apply fmap_Some in EVAL as (?&?&->).
-      destruct op; simpl in H; set_solver.
-    - destruct l0; try done. destruct op; try done. 
-      inversion EVAL. subst. 
-      repeat right. do 2 eexists. eauto.
-  Qed.
-
   Context (tok: iProp Σ).
   Context (si_add: execution_trace heap_lang -> iProp Σ).
   Context (PRES: tok_add_pres tok si_add).
   Context (τ: locale heap_lang).
   Local Notation interp' := (interp tok si_add τ). 
-
-  Ltac inv_binop_eval H :=
-    apply bin_op_eval_inv in H as
-        [(-> & ? & ->) | [(?&?&?&->&->&->&[(?&->) | (?&->)]&?) | [(?&?&?&->&->&->&?) | (?&?&->&->&->&->)]]].
 
   Lemma interp_binop_eval op n1 n2
     (NOLOC: forall l, n1 ≠ LitV (LitLoc l)):
@@ -70,22 +38,6 @@ Section typed_interp.
     5: set_solver.
     all: by rewrite interp_unfold. 
   Qed.
-
-  Lemma un_op_eval_inv op v r
-    (EVAL: un_op_eval op v = Some r):
-    (op = NegOp /\ exists b, v = LitV $ LitBool b /\ r = LitV $ LitBool $ negb b) \/
-    (op = NegOp /\ exists n, v = LitV $ LitInt n /\ r = LitV $ LitInt $ (Z.lnot n)) \/ 
-    (op = MinusUnOp /\ exists n, v = LitV $ LitInt n /\ r = LitV $ LitInt (- n)). 
-  Proof using All. 
-    rewrite /un_op_eval in EVAL.
-    destruct op, v; try congruence.
-    all: destruct l; try congruence; inversion EVAL; subst.
-    all: set_solver.
-  Qed.
-
-  Ltac inv_unop_eval H :=
-    apply un_op_eval_inv in H as
-        [(-> & ? & -> & ->) | [(-> & ? & -> & ->)| (-> & ? & -> & ->)]]. 
 
   Local Notation logrel' := (logrel tok si_add τ).
 
@@ -250,7 +202,11 @@ Section typed_interp.
     iApply wp_value. iFrame. 
 
     rewrite {3}interp_unfold.
-    inv_unop_eval EVAL; done. 
+    inv_unop_eval EVAL; try done.
+    destruct (val_into_int_spec v) as [(?&->&?) | (?&->)]; simpl.
+    - set_solver.
+    - iLeft. iExists _. iSplit; [done| ].
+      by rewrite {3}interp_unfold.
   Qed.
 
   Lemma logrel_binop op e1 e2
